Utils/Combinators.lean
@@ -1,0 +1,13 @@
+/-- Constant combinator -/
+def cI {α : Type} (a : α) : Unit -> α :=
+  fun _ ↦ a
+
+def mapToOption {α : Type} (p : Prop) [Decidable p] (f : Unit -> α) : Option α :=
+  if p then some (f ()) else none
+
+example : mapToOption (1 = 1) (cI 42) = some 42 := rfl
+
+def toSome {α : Type} (t : α) (p : Prop) [Decidable p] : Option α :=
+  if p then some t else none
+
+example : ((1 = 1) |> toSome 42) = some 42 := rfl
