Utils/Debug.lean
@@ -1,6 +1,6 @@
 
 /-- Asserts that two values `a` and `b` are equal. -/
-def assert_eq {T : Type} [BEq T] [ToString T] (s : String) (a b : T) : IO Unit := do
+def assert_eq {α : Type} [BEq α] [ToString α] (s : String) (a b : α) : IO Unit := do
   if a == b then
     IO.println s!"✅ Assertion: {s} == {b}"
   else
